Remove admits on memory invariants

src/lang/Memory.v
@@ -10,883 +10,11 @@ Require Import DataStructure.
 Require Import DenseOrder.
 Require Import Event.
 Require Import Time.
+Require Import View.
+Require Import Cell.
 
 Set Implicit Arguments.
 
-
-Module TimeMap <: JoinableType.
-  Definition t := Loc.t -> Time.t.
-
-  Definition eq := @eq t.
-
-  Definition le (lhs rhs:t): Prop :=
-    forall loc, Time.le (lhs loc) (rhs loc).
-
-  Global Program Instance le_PreOrder: PreOrder le.
-  Next Obligation. ii. refl. Qed.
-  Next Obligation. ii. etrans; eauto. Qed.
-
-  Definition bot: t := fun _ => Time.bot.
-
-  Lemma bot_spec (tm:t): le bot tm.
-  Proof. ii. apply Time.bot_spec. Qed.
-
-  Definition get (loc:Loc.t) (c:t) := c loc.
-
-  Definition join (lhs rhs:t): t :=
-    fun loc => Time.join (lhs loc) (rhs loc).
-
-  Lemma join_comm lhs rhs: join lhs rhs = join rhs lhs.
-  Proof. apply LocFun.ext. i. apply Time.join_comm. Qed.
-
-  Lemma join_assoc a b c: join (join a b) c = join a (join b c).
-  Proof.
-    apply LocFun.ext. i. apply Time.join_assoc.
-  Qed.
-
-  Lemma join_l lhs rhs: le lhs (join lhs rhs).
-  Proof. ii. apply Time.join_l. Qed.
-
-  Lemma join_r lhs rhs: le rhs (join lhs rhs).
-  Proof. ii. apply Time.join_r. Qed.
-
-  Lemma join_spec lhs rhs o
-        (LHS: le lhs o)
-        (RHS: le rhs o):
-    le (join lhs rhs) o.
-  Proof. unfold join. ii. apply Time.join_spec; auto. Qed.
-
-  Definition singleton loc ts :=
-    LocFun.add loc ts (LocFun.init Time.bot).
-
-  Lemma singleton_spec loc ts c
-        (LOC: Time.le ts (c loc)):
-    le (singleton loc ts) c.
-  Proof.
-    ii. unfold singleton, LocFun.add, LocFun.find.
-    condtac; subst; ss. apply Time.bot_spec.
-  Qed.
-
-  Lemma singleton_inv loc ts c
-        (LE: le (singleton loc ts) c):
-    Time.le ts (c loc).
-  Proof.
-    generalize (LE loc). unfold singleton, LocFun.add, LocFun.find.
-    condtac; [|congr]. auto.
-  Qed.
-
-  Lemma le_join_l l r
-        (LE: le r l):
-    join l r = l.
-  Proof.
-    apply LocFun.ext. i.
-    unfold join, Time.join, LocFun.find. condtac; auto.
-    apply TimeFacts.antisym; auto.
-  Qed.
-
-  Lemma le_join_r l r
-        (LE: le l r):
-    join l r = r.
-  Proof.
-    apply LocFun.ext. i.
-    unfold join, Time.join, LocFun.find. condtac; auto.
-    exfalso. eapply Time.lt_strorder. eapply TimeFacts.lt_le_lt; eauto.
-  Qed.
-
-  Lemma antisym l r
-        (LR: le l r)
-        (RL: le r l):
-    l = r.
-  Proof.
-    extensionality loc. apply TimeFacts.antisym; auto.
-  Qed.
-End TimeMap.
-
-Module Capability <: JoinableType.
-  Structure t_ := mk {
-    ur: TimeMap.t;
-    rw: TimeMap.t;
-    sc: TimeMap.t;
-  }.
-  Definition t := t_.
-
-  Inductive wf (capability:t): Prop :=
-  | wf_intro
-      (UR_RW: TimeMap.le capability.(ur) capability.(rw))
-      (RW_SC: TimeMap.le capability.(rw) capability.(sc))
-  .
-
-  Definition eq := @eq t.
-
-  Inductive le_ (lhs rhs:t): Prop :=
-  | le_intro
-      (UR: TimeMap.le lhs.(ur) rhs.(ur))
-      (RW: TimeMap.le lhs.(rw) rhs.(rw))
-      (SC: TimeMap.le lhs.(sc) rhs.(sc))
-  .
-  Definition le := le_.
-
-  Global Program Instance le_PreOrder: PreOrder le.
-  Next Obligation.
-    ii. econs; refl.
-  Qed.
-  Next Obligation.
-    ii. inv H. inv H0. econs; etrans; eauto.
-  Qed.
-
-  Lemma ext l r
-        (UR: l.(ur) = r.(ur))
-        (RW: l.(rw) = r.(rw))
-        (SC: l.(sc) = r.(sc)):
-    l = r.
-  Proof.
-    destruct l, r. f_equal; auto.
-  Qed.
-
-  Definition bot: t := mk TimeMap.bot TimeMap.bot TimeMap.bot.
-
-  Lemma bot_wf: wf bot.
-  Proof. econs; refl. Qed.
-
-  Lemma bot_spec (c:t): le bot c.
-  Proof. econs; apply TimeMap.bot_spec. Qed.
-
-  Definition join (lhs rhs:t): t :=
-    mk (TimeMap.join lhs.(ur) rhs.(ur))
-       (TimeMap.join lhs.(rw) rhs.(rw))
-       (TimeMap.join lhs.(sc) rhs.(sc)).
-
-  Lemma join_comm lhs rhs: join lhs rhs = join rhs lhs.
-  Proof. unfold join. f_equal; apply TimeMap.join_comm. Qed.
-
-  Lemma join_assoc a b c: join (join a b) c = join a (join b c).
-  Proof.
-    unfold join. ss. f_equal.
-    - apply TimeMap.join_assoc.
-    - apply TimeMap.join_assoc.
-    - apply TimeMap.join_assoc.
-  Qed.
-
-  Lemma join_l lhs rhs: le lhs (join lhs rhs).
-  Proof. econs; apply TimeMap.join_l. Qed.
-
-  Lemma join_r lhs rhs: le rhs (join lhs rhs).
-  Proof. econs; apply TimeMap.join_r. Qed.
-
-  Lemma join_spec lhs rhs o
-        (LHS: le lhs o)
-        (RHS: le rhs o):
-    le (join lhs rhs) o.
-  Proof.
-    inv LHS. inv RHS.
-    econs; apply TimeMap.join_spec; eauto.
-  Qed.
-
-  Lemma join_wf
-        lhs rhs
-        (LHS: wf lhs)
-        (RHS: wf rhs):
-    wf (join lhs rhs).
-  Proof.
-    econs.
-    - apply TimeMap.join_spec.
-      + etrans; [apply LHS|]. apply TimeMap.join_l.
-      + etrans; [apply RHS|]. apply TimeMap.join_r.
-    - apply TimeMap.join_spec.
-      + etrans; [apply LHS|]. apply TimeMap.join_l.
-      + etrans; [apply RHS|]. apply TimeMap.join_r.
-  Qed.
-
-  Definition bot_unless (cond:bool) (c:t): t :=
-    if cond then c else bot.
-
-  Lemma bot_unless_wf
-        cond c
-        (WF: wf c):
-    wf (bot_unless cond c).
-  Proof.
-    destruct cond; ss. apply bot_wf.
-  Qed.
-
-  Definition singleton_ur loc ts :=
-    mk (TimeMap.singleton loc ts)
-       (TimeMap.singleton loc ts)
-       (TimeMap.singleton loc ts).
-
-  Lemma singleton_ur_wf
-        loc ts:
-    wf (singleton_ur loc ts).
-  Proof.
-    econs; ss; refl.
-  Qed.
-
-  Lemma singleton_ur_spec loc ts c
-        (WF: wf c)
-        (TS: Time.le ts (c.(ur) loc)):
-    le (singleton_ur loc ts) c.
-  Proof.
-    econs; s;
-      try apply TimeMap.bot_spec;
-      try apply TimeMap.singleton_spec; auto.
-    - etrans; eauto. apply WF.
-    - etrans; eauto. etrans; apply WF.
-  Qed.
-
-  Lemma singleton_ur_inv loc ts c
-        (LE: le (singleton_ur loc ts) c):
-    Time.le ts (c.(ur) loc).
-  Proof.
-    apply TimeMap.singleton_inv. apply LE.
-  Qed.
-
-  Definition singleton_rw loc ts :=
-    mk TimeMap.bot
-       (TimeMap.singleton loc ts)
-       (TimeMap.singleton loc ts).
-
-  Lemma singleton_rw_wf
-        loc ts:
-    wf (singleton_rw loc ts).
-  Proof.
-    econs; ss; try refl. apply TimeMap.bot_spec.
-  Qed.
-
-  Lemma singleton_rw_spec loc ts c
-        (WF: wf c)
-        (TS: Time.le ts (c.(rw) loc)):
-    le (singleton_rw loc ts) c.
-  Proof.
-    econs; s;
-      try apply TimeMap.bot_spec;
-      try apply TimeMap.singleton_spec; auto.
-    etrans; eauto. apply WF.
-  Qed.
-
-  Lemma singleton_rw_inv loc ts c
-        (LE: le (singleton_rw loc ts) c):
-    Time.le ts (c.(rw) loc).
-  Proof.
-    apply TimeMap.singleton_inv. apply LE.
-  Qed.
-
-  Definition singleton_sc loc ts :=
-    mk TimeMap.bot
-       TimeMap.bot
-       (TimeMap.singleton loc ts).
-
-  Lemma singleton_sc_wf
-        loc ts:
-    wf (singleton_sc loc ts).
-  Proof.
-    econs; ss; try refl. apply TimeMap.bot_spec.
-  Qed.
-
-  Lemma singleton_sc_spec loc ts c
-        (WF: wf c)
-        (TS: Time.le ts (c.(sc) loc)):
-    le (singleton_sc loc ts) c.
-  Proof.
-    econs; s;
-      try apply TimeMap.bot_spec;
-      try apply TimeMap.singleton_spec; auto.
-  Qed.
-
-  Lemma singleton_sc_inv loc ts c
-        (LE: le (singleton_sc loc ts) c):
-    Time.le ts (c.(sc) loc).
-  Proof.
-    apply TimeMap.singleton_inv. apply LE.
-  Qed.
-
-  Lemma le_join_l l r
-        (LE: le r l):
-    join l r = l.
-  Proof.
-    unfold join. destruct l. ss.
-    f_equal; apply TimeMap.le_join_l; apply LE.
-  Qed.
-
-  Lemma le_join_r l r
-        (LE: le l r):
-    join l r = r.
-  Proof.
-    unfold join. destruct r. ss.
-    f_equal; apply TimeMap.le_join_r; apply LE.
-  Qed.
-
-  Lemma antisym l r
-        (LR: le l r)
-        (RL: le r l):
-    l = r.
-  Proof.
-    destruct l, r. inv LR. inv RL. ss. f_equal.
-    - apply TimeMap.antisym; auto.
-    - apply TimeMap.antisym; auto.
-    - apply TimeMap.antisym; auto.
-  Qed.
-
-  Lemma timemap_le_le tm1 tm2
-        (LE: TimeMap.le tm1 tm2):
-    le (mk tm1 tm1 tm1) (mk tm2 tm2 tm2).
-  Proof. econs; eauto. Qed.
-End Capability.
-
-Module Message.
-  Structure t := mk {
-    val: Const.t;
-    released: Capability.t;
-  }.
-  Definition elt: t := mk 0 Capability.bot.
-End Message.
-
-Module Cell.
-  Module Raw.
-    Definition t := DOMap.t (DenseOrder.t * Message.t).
-
-    Inductive wf (cell:t): Prop :=
-    | wf_intro
-        (VOLUME: forall from to msg
-                   (GET: DOMap.find to cell = Some (from, msg)),
-            (from, to) = (Time.bot, Time.bot) \/ Time.lt from to)
-        (DISJOINT: forall to1 to2 from1 from2 msg1 msg2
-                     (GET1: DOMap.find to1 cell = Some (from1, msg1))
-                     (GET2: DOMap.find to2 cell = Some (from2, msg2))
-                     (NEQ: to1 <> to2),
-            Interval.disjoint (from1, to1) (from2, to2))
-    .
-
-    Definition bot: t := DOMap.empty _.
-
-    Lemma bot_wf: wf bot.
-    Proof.
-      econs; i.
-      - rewrite DOMap.gempty in GET. inv GET.
-      - rewrite DOMap.gempty in GET1. inv GET1.
-    Qed.
-
-    Definition singleton (from to:Time.t) (val:Const.t) (released:Capability.t): t :=
-      DOMap.singleton to (from, Message.mk val released).
-
-    Lemma singleton_wf
-          from to val released
-          (LT: Time.lt from to):
-      wf (singleton from to val released).
-    Proof.
-      unfold singleton. econs; s; i.
-      - apply DOMap.singleton_find_inv in GET. des. inv GET0.
-        auto.
-      - apply DOMap.singleton_find_inv in GET1. des. inv GET0.
-        apply DOMap.singleton_find_inv in GET2. des. inv GET0.
-        congr.
-    Qed.
-
-    Definition init: t :=
-      DOMap.singleton Time.bot (Time.bot, Message.mk 0 Capability.bot).
-
-    Lemma init_wf: wf init.
-    Proof.
-      unfold init. econs; s; i.
-      - apply DOMap.singleton_find_inv in GET. des. inv GET0.
-        auto.
-      - apply DOMap.singleton_find_inv in GET1. des. inv GET0.
-        apply DOMap.singleton_find_inv in GET2. des. inv GET0.
-        congr.
-    Qed.
-
-    Lemma find_mem_ub
-          from to msg cell
-          (WF: wf cell)
-          (FIND: DOMap.find to cell = Some (from, msg)):
-      (from, to) = (Time.bot, Time.bot) \/
-      Interval.mem (from, to) to.
-    Proof.
-      inv WF. exploit VOLUME; eauto. i. des; auto.
-      right. econs; eauto. refl.
-    Qed.
-
-    Inductive add (cell1:t) (from to:Time.t) (val:Const.t) (released:Capability.t): forall (rhs:t), Prop :=
-    | add_intro
-        (DISJOINT: forall to2 from2 msg2
-                     (GET2: DOMap.find to2 cell1 = Some (from2, msg2)),
-            to <> from2 /\ Interval.disjoint (from, to) (from2, to2))
-        (TO1: Time.lt from to):
-        add cell1 from to val released (DOMap.add to (from, (Message.mk val released)) cell1)
-    .
-
-    Lemma add_wf
-          cell1 from to val released rhs
-          (ADD: add cell1 from to val released rhs)
-          (CELL1: wf cell1):
-      wf rhs.
-    Proof.
-      inv ADD. inv CELL1. econs; i.
-      - rewrite DOMap.Facts.add_o in *.
-        revert GET. condtac; i.
-        + inv GET. auto.
-        + eapply VOLUME. eauto.
-      - rewrite DOMap.Facts.add_o in *.
-        revert GET1 GET2. repeat condtac; i; repeat subst.
-        + congr.
-        + inv GET1. eapply DISJOINT; eauto.
-        + inv GET2. symmetry. eapply DISJOINT; eauto.
-        + eapply DISJOINT0; eauto.
-    Qed.
-
-    Inductive split (cell1:t) (from to1 to2:Time.t) (val1:Const.t) (released1:Capability.t): forall (rhs:t), Prop :=
-    | split_intro
-        msg2
-        (GET2: DOMap.find to2 cell1 = Some (from, msg2))
-        (TO1: Time.lt from to1)
-        (TO2: Time.lt to1 to2):
-        split cell1 from to1 to2 val1 released1
-              (DOMap.add to1 (from, Message.mk val1 released1) (DOMap.add to2 (to1, msg2) cell1))
-    .
-
-    Lemma split_wf
-          cell1 from1 to1 to2 val1 released1 cell2
-          (SPLIT: split cell1 from1 to1 to2 val1 released1 cell2)
-          (CELL1: wf cell1):
-      wf cell2.
-    Proof.
-      inv SPLIT. inv CELL1. econs; i.
-      - rewrite ? DOMap.Facts.add_o in *.
-        revert GET. repeat condtac; i; try by inv GET; auto.
-        eapply VOLUME. eauto.
-      - rewrite ? DOMap.Facts.add_o in *.
-        revert GET1 GET0. repeat condtac; i; repeat subst; try congr;
-          (repeat match goal with
-                 | [H: Some _ = Some _ |- _] => inv H
-                  end);
-          (try by eapply DISJOINT; eauto).
-        + apply Interval.disjoint_imm.
-        + ii. eapply (DISJOINT to3 to2); eauto.
-          eapply Interval.le_mem; try apply LHS.
-          econs; s. refl. apply Time.le_lteq. auto.
-        + symmetry. apply Interval.disjoint_imm.
-        + ii. eapply (DISJOINT to3 to0); eauto.
-          eapply Interval.le_mem; try apply LHS.
-          econs; s. apply Time.le_lteq. auto. refl.
-        + ii. eapply (DISJOINT to0 to2); eauto.
-          eapply Interval.le_mem; try apply RHS.
-          econs; s. refl. apply Time.le_lteq. auto.
-        + ii. eapply (DISJOINT to0 to3); eauto.
-          eapply Interval.le_mem; try apply RHS.
-          econs; s. apply Time.le_lteq. auto. refl.
-    Qed.
-
-    Inductive remove (cell1:t) (from to:Time.t) (val:Const.t) (released:Capability.t): forall (rhs:t), Prop :=
-    | remove_intro
-        (GET: DOMap.find to cell1 = Some (from, Message.mk val released)):
-        remove cell1 from to val released (DOMap.remove to cell1)
-    .
-
-    Lemma remove_wf
-          cell1 from to val released rhs
-          (REMOVE: remove cell1 from to val released rhs)
-          (CELL1: wf cell1):
-      wf rhs.
-    Proof.
-      inv REMOVE. inv CELL1. econs; i.
-      - revert GET0. rewrite DOMap.Facts.remove_o.
-        condtac; eauto. congr.
-      - revert GET1 GET2. rewrite ? DOMap.Facts.remove_o.
-        repeat condtac; i; try congr.
-        eapply DISJOINT; eauto.
-    Qed.
-  End Raw.
-
-  Structure t := mk {
-    raw :> Raw.t;
-    WF: Raw.wf raw;
-  }.
-
-  Definition get (ts:Time.t) (cell:t): option (Time.t * Message.t) := DOMap.find ts cell.(raw).
-
-  Lemma ext
-        (lhs rhs:t)
-        (EXT: forall ts, get ts lhs = get ts rhs):
-    lhs = rhs.
-  Proof.
-    destruct lhs, rhs.
-    assert (raw0 = raw1).
-    { apply DOMap.eq_leibniz. ii. apply EXT. }
-    subst raw1. f_equal. apply proof_irrelevance.
-  Qed.
-
-  Definition le (lhs rhs:t): Prop :=
-    forall to from msg
-      (LHS: get to lhs = Some (from, msg)),
-      get to rhs = Some (from, msg).
-
-  Global Program Instance le_PreOrder: PreOrder le.
-  Next Obligation. ii. auto. Qed.
-  Next Obligation. ii. eapply H0; eauto. Qed.
-
-  Inductive disjoint (lhs rhs:t): Prop :=
-  | disjoint_intro
-      (DISJOINT0: forall from1 from2 msg1 msg2
-                    (GET1: get Time.bot lhs = Some (from1, msg1))
-                    (GET2: get Time.bot rhs = Some (from2, msg2)),
-          False)
-      (DISJOINT1: forall to1 to2 from1 from2 msg1 msg2
-                    (GET1: get to1 lhs = Some (from1, msg1))
-                    (GET2: get to2 rhs = Some (from2, msg2)),
-          Interval.disjoint (from1, to1) (from2, to2))
-  .
-
-  Global Program Instance disjoint_Symmetric: Symmetric disjoint.
-  Next Obligation.
-    inv H. econs.
-    - i. eapply DISJOINT0; eauto.
-    - i. symmetry. eapply DISJOINT1; eauto.
-  Qed.
-
-  Lemma disjoint_get
-        lhs rhs
-        ts lmsg rmsg
-        (DISJOINT: disjoint lhs rhs)
-        (LMSG: get ts lhs = Some lmsg)
-        (RMSG: get ts rhs = Some rmsg):
-    False.
-  Proof.
-    destruct lmsg, rmsg. unfold get in *.
-    destruct (DOMap.find ts lhs.(raw)) as [[]|] eqn:LHS; inv LMSG.
-    destruct (DOMap.find ts rhs.(raw)) as [[]|] eqn:RHS; inv RMSG.
-    exploit Raw.find_mem_ub; try apply lhs; eauto. i.
-    exploit Raw.find_mem_ub; try apply rhs; eauto. i.
-    inv DISJOINT. des; inversion x0; inversion x1; subst; try by inv FROM.
-    - eapply DISJOINT0; eauto.
-    - eapply DISJOINT1; eauto.
-  Qed.
-
-  Definition bot: t := mk Raw.bot_wf.
-
-  Lemma bot_get ts: get ts bot = None.
-  Proof. unfold get, bot, Raw.bot. s. apply DOMap.gempty. Qed.
-
-  Lemma bot_le cell: le bot cell.
-  Proof. ii. rewrite bot_get in LHS. congr. Qed.
-
-  Lemma bot_disjoint cell: disjoint bot cell.
-  Proof.
-    econs.
-    - ii. rewrite bot_get in GET1. congr.
-    - i. rewrite bot_get in GET1. congr.
-  Qed.
-
-  Definition singleton
-             (from to:Time.t) (val:Const.t) (released:Capability.t)
-             (LT: Time.lt from to): t :=
-    mk (Raw.singleton_wf val released LT).
-
-  Lemma singleton_get
-        from to val released (LT:Time.lt from to)
-        t:
-    get t (singleton val released LT) =
-    if Loc.eq_dec t to
-    then Some (from, Message.mk val released)
-    else None.
-  Proof.
-    unfold get, singleton, Raw.singleton. ss. condtac.
-    - subst. rewrite DOMap.singleton_eq. auto.
-    - rewrite DOMap.singleton_neq; auto.
-  Qed.
-
-  Definition init: t := mk Raw.init_wf.
-
-  Definition add (cell1:t) (from1 to1:Time.t) (val1:Const.t) (released1:Capability.t) (cell2:t): Prop :=
-    Raw.add cell1 from1 to1 val1 released1 cell2.
-
-  Definition split (cell1:t) (from1 to1 to2:Time.t) (val1:Const.t) (released1:Capability.t) (cell2:t): Prop :=
-    Raw.split cell1 from1 to1 to2 val1 released1 cell2.
-
-  Definition remove (cell1:t) (from1 to1:Time.t) (val1:Const.t) (released1:Capability.t) (cell2:t): Prop :=
-    Raw.remove cell1 from1 to1 val1 released1 cell2.
-
-  Definition max_ts (cell:t): Time.t :=
-    DOMap.max_key _ cell.(raw).
-
-  Lemma max_ts_spec
-        ts from msg cell
-        (GET: get ts cell = Some (from, msg)):
-    <<GET: exists from val released, get (max_ts cell) cell = Some (from, Message.mk val released)>> /\
-    <<MAX: Time.le ts (max_ts cell)>>.
-  Proof.
-    unfold get in GET.
-    generalize (DOMap.max_key_spec _ cell.(Cell.raw)). i. des. splits; eauto.
-    - destruct (DOMap.find
-                  (DOMap.max_key (DenseOrder.t * Message.t) (Cell.raw cell))
-                  (Cell.raw cell)) as [[? []]|] eqn:X.
-      + esplits. eauto.
-      + exfalso. eapply FIND; eauto. rewrite GET. congr.
-    - apply MAX. rewrite GET. auto. congr.
-  Qed.
-
-  Lemma add_exists
-        cell1 from to val released
-        (DISJOINT: forall to2 from2 msg2
-                     (GET2: get to2 cell1 = Some (from2, msg2)),
-            to <> from2 /\ Interval.disjoint (from, to) (from2, to2))
-        (TO1: Time.lt from to):
-    exists cell2, add cell1 from to val released cell2.
-  Proof.
-    destruct cell1. eexists (mk _). unfold add. econs; eauto.
-  Grab Existential Variables.
-    eapply Raw.add_wf; eauto. econs; eauto.
-  Qed.
-
-  Lemma add_exists_max_ts
-        cell1 to val released
-        (TO: Time.lt (max_ts cell1) to)
-        (WF: Capability.wf released):
-    exists cell2, add cell1 (max_ts cell1) to val released cell2.
-  Proof.
-    apply add_exists; auto. i.
-    exploit max_ts_spec; eauto. i. des. splits.
-    - ii. subst. destruct cell1.(Cell.WF). exploit VOLUME; try apply GET2; eauto. i. des.
-      + inv x. inv TO.
-      + rewrite x in TO. eapply Time.lt_strorder. eapply TimeFacts.le_lt_lt; eauto.
-    - ii. inv LHS. inv RHS. ss.
-      rewrite MAX in TO1. eapply Time.lt_strorder. eapply TimeFacts.le_lt_lt; eauto.
-  Qed.
-
-  Lemma add_exists_le
-        promises1 cell1 from to val released cell2
-        (LE: le promises1 cell1)
-        (ADD: add cell1 from to val released cell2):
-    exists promises2, add promises1 from to val released promises2.
-  Proof.
-    inv ADD. apply add_exists; auto. i.
-    eapply DISJOINT. eauto.
-  Qed.
-
-  Lemma split_exists
-        cell1 from to1 to2 val released msg2
-        (GET2: get to2 cell1 = Some (from, msg2))
-        (TO1: Time.lt from to1)
-        (TO2: Time.lt to1 to2):
-    exists cell2, split cell1 from to1 to2 val released cell2.
-  Proof.
-    destruct cell1. eexists (mk _). unfold split. econs; eauto.
-  Grab Existential Variables.
-    eapply Raw.split_wf; eauto. econs; eauto.
-  Qed.
-
-  Lemma split_exists_le
-        promises1 cell1 from to1 to2 val released promises2
-        (LE: le promises1 cell1)
-        (SPLIT: split promises1 from to1 to2 val released promises2):
-    exists cell2, split cell1 from to1 to2 val released cell2.
-  Proof.
-    inv SPLIT. eapply split_exists; eauto.
-  Qed.
-
-  (* Lemmas on add, split & remove *)
-
-  Lemma add_disjoint
-        cell1 from1 to1 val1 released1 cell2
-        (ADD: add cell1 from1 to1 val1 released1 cell2):
-    get to1 cell1 = None.
-  Proof.
-    inv ADD. unfold get.
-    destruct (DOMap.find to1 (raw cell1)) as [[]|] eqn:X; auto.
-    exfalso. exploit DISJOINT; eauto. i. des.
-    eapply x0.
-    - apply Interval.mem_ub. auto.
-    - apply Interval.mem_ub.
-      destruct cell1.(Cell.WF). exploit VOLUME; eauto. i. des; ss.
-      inv x1. congr.
-  Qed.
-
-  Lemma add_get1
-        cell1 from1 to1 val1 released1 cell2
-        t f m
-        (ADD: add cell1 from1 to1 val1 released1 cell2)
-        (GET: get t cell1 = Some (f, m)):
-    get t cell2 = Some (f, m).
-  Proof.
-    exploit add_disjoint; eauto. i.
-    unfold get in *. inv ADD.
-    rewrite DOMap.gsspec. condtac; auto. subst.
-    congr.
-  Qed.
-
-  Lemma add_get2
-        cell1 from1 to1 val1 released1 cell2
-        (ADD: add cell1 from1 to1 val1 released1 cell2):
-    get to1 cell2 = Some (from1, Message.mk val1 released1).
-  Proof.
-    unfold get in *. inv ADD.
-    rewrite DOMap.gss. auto.
-  Qed.
-
-  Lemma add_get_inv
-        cell1 from1 to1 val1 released1 cell2
-        t f m
-        (ADD: add cell1 from1 to1 val1 released1 cell2)
-        (GET: get t cell2 = Some (f, m)):
-    (t = to1 /\ f = from1 /\ m = Message.mk val1 released1) \/
-    (~ t = to1 /\
-     get t cell1 = Some (f, m)).
-  Proof.
-    unfold get in *. inv ADD.
-    revert GET. rewrite <- H0. rewrite DOMap.gsspec. condtac; auto.
-    i. inv GET. auto.
-  Qed.
-
-  Lemma add_inhabited
-        cell1 cell2 from to val released
-        (ADD: add cell1 from to val released cell2)
-        (INHABITED: get Time.bot cell1 = Some (Time.bot, Message.elt)):
-    <<INHABITED: get Time.bot cell2 = Some (Time.bot, Message.elt)>>.
-  Proof.
-    des. exploit add_get1; eauto.
-  Qed.
-
-  Lemma add_max_ts
-        cell1 to val released cell2
-        (INHABITED: get Time.bot cell1 = Some (Time.bot, Message.elt))
-        (ADD: add cell1 (max_ts cell1) to val released cell2):
-    max_ts cell2 = to.
-  Proof.
-    hexploit add_inhabited; eauto. i. des.
-    exploit max_ts_spec; eauto. i. des.
-    apply TimeFacts.antisym.
-    - exploit add_get_inv; eauto. i. des.
-      + subst. refl.
-      + left. eapply TimeFacts.le_lt_lt.
-        * eapply max_ts_spec. rewrite x1. eauto.
-        * inv ADD. eauto.
-    - eapply max_ts_spec. erewrite add_get2; eauto.
-  Qed.
-
-  Lemma split_disjoint
-        cell1 from1 to1 to2 val1 released1 cell2
-        (SPLIT: split cell1 from1 to1 to2 val1 released1 cell2):
-    get to1 cell1 = None.
-  Proof.
-    unfold get in *. destruct cell1, cell2. inv SPLIT. ss. subst.
-    destruct (DOMap.find to1 raw0) as [[]|] eqn:X; [|done].
-    exfalso. inv WF0. eapply DISJOINT; [apply GET2|apply X| | |].
-    - ii. subst. eapply Time.lt_strorder. eauto.
-    - econs; eauto. apply Time.le_lteq. auto.
-    - apply Interval.mem_ub.
-      exploit VOLUME; eauto. i. des; ss.
-      inv x. inv TO1.
-  Qed.
-
-  Lemma split_get0
-        cell1 from1 to1 to2 val1 released1 cell2
-        (SPLIT: split cell1 from1 to1 to2 val1 released1 cell2):
-    exists msg2, get to2 cell1 = Some (from1, msg2).
-  Proof.
-    inv SPLIT. eauto.
-  Qed.
-
-  Lemma split_get1
-        cell1 from1 to1 to2 val1 released1 cell2
-        t f m
-        (SPLIT: split cell1 from1 to1 to2 val1 released1 cell2)
-        (GET: get t cell1 = Some (f, m)):
-    (f = from1 /\ t = to2 /\ get t cell2 = Some (to1, m)) \/
-    (~ (t = to2) /\
-     get t cell2 = Some (f, m)).
-  Proof.
-    unfold get in *. destruct cell1, cell2. inv SPLIT. ss. subst.
-    rewrite ? DOMap.gsspec. repeat condtac; subst; ss.
-    - destruct WF0.
-      exfalso. eapply DISJOINT; [apply GET2|apply GET| | |].
-      + ii. subst. eapply Time.lt_strorder. eauto.
-      + econs; eauto. apply Time.le_lteq. auto.
-      + apply Interval.mem_ub.
-        exploit VOLUME; eauto. i. des; ss.
-        inv x. inv TO1.
-    - rewrite GET2 in *. inv GET. eauto.
-    - rewrite GET. right. splits; eauto.
-  Qed.
-
-  Lemma split_get1'
-        cell1 from1 to1 to2 val1 released1 cell2
-        t f m
-        (SPLIT: split cell1 from1 to1 to2 val1 released1 cell2)
-        (GET: get t cell1 = Some (f, m)):
-    exists f', get t cell2 = Some (f', m).
-  Proof.
-    exploit split_get1; eauto. i. des; eauto.
-  Qed.
-
-  Lemma split_get2
-        cell1 from1 to1 to2 val1 released1 cell2
-        (SPLIT: split cell1 from1 to1 to2 val1 released1 cell2):
-    get to1 cell2 = Some (from1, Message.mk val1 released1).
-  Proof.
-    unfold get in *. destruct cell1, cell2. inv SPLIT. ss. subst.
-    apply DOMap.gss.
-  Qed.
-
-  Lemma split_get_inv
-        cell1 from1 to1 to2 val1 released1 cell2
-        t f m
-        (SPLIT: split cell1 from1 to1 to2 val1 released1 cell2)
-        (GET: get t cell2 = Some (f, m)):
-    (t = to1 /\ f = from1 /\ m = Message.mk val1 released1) \/
-    (t = to2 /\ f = to1 /\ get t cell1 = Some (from1, m)) \/
-    (~ (t = to1) /\
-     ~ (t = to2) /\
-     get t cell1 = Some (f, m)).
-  Proof.
-    unfold get in *. destruct cell1, cell2. inv SPLIT. ss. subst.
-    revert GET. rewrite ? DOMap.gsspec. repeat condtac; subst; i; inv GET; auto.
-  Qed.
-
-  Lemma split_get_inv'
-        cell1 from1 to1 to2 val1 released1 cell2
-        t f m
-        (SPLIT: split cell1 from1 to1 to2 val1 released1 cell2)
-        (GET: get t cell2 = Some (f, m)):
-    (t = to1 /\ f = from1 /\ m = Message.mk val1 released1) \/ exists f', get t cell1 = Some (f', m).
-  Proof.
-    exploit split_get_inv; eauto. i. des; eauto.
-  Qed.
-
-  Lemma split_inhabited
-        cell1 cell2 from to1 to2 val released
-        (SPLIT: split cell1 from to1 to2 val released cell2)
-        (INHABITED: get Time.bot cell1 = Some (Time.bot, Message.elt)):
-    <<INHABITED: get Time.bot cell2 = Some (Time.bot, Message.elt)>>.
-  Proof.
-    des. exploit split_get1; eauto. i. des; auto.
-    subst. inv SPLIT. inv TO2.
-  Qed.
-
-  Lemma remove_singleton
-        from to val released (LT:Time.lt from to):
-    remove (singleton val released LT) from to val released bot.
-  Proof.
-    assert (Raw.bot = DOMap.remove to ((singleton val released LT).(raw))).
-    { apply DOMap.eq_leibniz. ii.
-      unfold Raw.bot. rewrite DOMap.gempty.
-      rewrite DOMap.grspec. condtac; auto.
-      unfold singleton, Raw.singleton, raw.
-      rewrite DOMap.singleton_neq; auto.
-    }
-    unfold remove. s. rewrite H. econs. s.
-    unfold Raw.singleton. rewrite DOMap.singleton_eq. auto.
-  Qed.
-
-  Lemma remove_exists
-        cell1 from to val released
-        (GET: get to cell1 = Some (from, Message.mk val released)):
-    exists cell2, remove cell1 from to val released cell2.
-  Proof.
-    eexists (mk _). destruct cell1. ss.
-    Grab Existential Variables.
-    { eapply Raw.remove_wf.
-      - econs. eauto.
-      - apply WF.
-    }
-  Qed.
-End Cell.
 
 Module Memory.
   Definition t := Loc.t -> Cell.t.
@@ -1090,21 +218,18 @@ Module Memory.
   | promise_add
       (PROMISES: add promises1 loc from1 to1 val1 released1 promises2)
       (MEM: add mem1 loc from1 to1 val1 released1 mem2)
-      (CLOSED: closed_capability released1 mem2)
       (TS: Time.le (Capability.rw released1 loc) to1):
       promise promises1 mem1 loc from1 to1 val1 released1 promises2 mem2 promise_kind_add
   | promise_split
       to2
       (PROMISES: split promises1 loc from1 to1 to2 val1 released1 promises2)
       (MEM: split mem1 loc from1 to1 to2 val1 released1 mem2)
-      (CLOSED: closed_capability released1 mem2)
       (TS: Time.le (Capability.rw released1 loc) to1):
       promise promises1 mem1 loc from1 to1 val1 released1 promises2 mem2 promise_kind_split
   | promise_lower
       released0
       (PROMISES: lower promises1 loc from1 to1 val1 released0 released1 promises2)
-      (MEM: lower mem1 loc from1 to1 val1 released0 released1 mem2)
-      (CLOSED: closed_capability released1 mem2):
+      (MEM: lower mem1 loc from1 to1 val1 released0 released1 mem2):
       promise promises1 mem1 loc from1 to1 val1 released1 promises2 mem2 promise_kind_lower
   .
 
@@ -1703,13 +828,13 @@ Module Memory.
         eexists. eauto.
   Qed.
 
-  Lemma promise_future
+  Lemma promise_future0
         promises1 mem1 loc from to val released promises2 mem2 kind
         (LE_PROMISES1: le promises1 mem1)
-        (CLOSED1: closed mem1)
+        (INHABITED1: inhabited mem1)
         (PROMISE: promise promises1 mem1 loc from to val released promises2 mem2 kind):
     <<LE_PROMISES2: le promises2 mem2>> /\
-    <<CLOSED2: closed mem2>> /\
+    <<INHABITED2: inhabited mem2>> /\
     <<FUTURE: future mem1 mem2>>.
   Proof.
     inv PROMISE.
@@ -1717,54 +842,62 @@ Module Memory.
       + ii. eapply add_get_inv in LHS; eauto. des.
         * subst. eapply add_get2. eauto.
         * eapply add_get1; eauto.
-      + econs.
-        * ii. eapply add_get_inv in MSG; eauto. des.
-          { inv MSG2. inv MEM. eauto. }
-          { inv CLOSED1. exploit CLOSED0; eauto. i. des. splits; auto.
-            eapply future_closed_capability; eauto.
-            econs 2; eauto. econs 1. eauto.
-          }
-        * eapply add_inhabited; eauto. apply CLOSED1.
+      + eapply add_inhabited; eauto.
       + econs 2; eauto. econs 1; eauto.
     - splits; eauto.
       + ii. eapply split_get_inv in LHS; eauto. des.
         * subst. eapply split_get2. eauto.
-        * subst. exploit split_get1; try apply MEM; eauto. i. des; auto.
+        * subst. exploit split_get1; try apply MEM; try apply LE_PROMISES1; eauto. i. des; auto.
           contradict x0. auto.
-        * exploit split_get1; try apply MEM; eauto. i. des; auto.
+        * exploit split_get1; try apply MEM; try apply LE_PROMISES1; eauto. i. des; auto.
           subst. contradict LHS0. auto.
-      + econs.
-        * ii. eapply split_get_inv' in MSG; eauto. des.
-          { inv MSG2. inv MEM. eauto. }
-          { inv CLOSED1. exploit CLOSED0; eauto. i. des. splits; auto.
-            eapply future_closed_capability; eauto.
-            econs 2; eauto. econs 2. eauto.
-          }
-        * eapply split_inhabited; eauto. apply CLOSED1.
+      + eapply split_inhabited; eauto.
       + econs 2; eauto. econs 2; eauto.
     - splits; eauto.
       + ii. eapply lower_get_inv in LHS; eauto. des.
         * subst. eapply lower_get2. eauto.
         * exploit lower_get1; try apply MEM; eauto. i. rewrite <- x0. auto.
-      + econs.
-        * ii. eapply lower_get_inv in MSG; eauto. des.
-          { inv MSG2. splits; eauto.
-            - inv MEM. inv ADD. auto.
-            - inv MEM. etrans; [eapply LE|].
-              eapply CLOSED1. eapply remove_get0. eauto.
-          }
-          { inv CLOSED1. exploit CLOSED0; eauto. i. des. splits; auto.
-            eapply future_closed_capability; eauto.
-            econs 2; eauto. econs 3. eauto.
-          }
-        * eapply lower_inhabited; eauto. apply CLOSED1.
+      + eapply lower_inhabited; eauto.
       + econs 2; eauto. econs 3; eauto.
+  Qed.
+
+  Lemma promise_future
+        promises1 mem1 loc from to val released promises2 mem2 kind
+        (LE_PROMISES1: le promises1 mem1)
+        (CLOSED1: closed mem1)
+        (CLOSED_REL: closed_capability released mem2)
+        (PROMISE: promise promises1 mem1 loc from to val released promises2 mem2 kind):
+    <<LE_PROMISES2: le promises2 mem2>> /\
+    <<CLOSED2: closed mem2>> /\
+    <<FUTURE: future mem1 mem2>>.
+  Proof.
+    exploit promise_future0; try apply CLOSED1; eauto. i. des. splits; auto.
+    inv PROMISE.
+    - econs; eauto.
+      ii. eapply add_get_inv in MSG; eauto. des.
+      + inv MSG2. inv MEM. eauto.
+      + inv CLOSED1. exploit CLOSED; eauto. i. des. splits; auto.
+        eapply future_closed_capability; eauto.
+    - econs; eauto.
+      ii. eapply split_get_inv' in MSG; eauto. des.
+      + inv MSG2. inv MEM. eauto.
+      + inv CLOSED1. exploit CLOSED; eauto. i. des. splits; auto.
+        eapply future_closed_capability; eauto.
+    - econs; eauto.
+      ii. eapply lower_get_inv in MSG; eauto. des.
+      + inv MSG2. splits; eauto.
+        * inv MEM. inv ADD. auto.
+        * inv MEM. etrans; [eapply LE|].
+          eapply CLOSED1. eapply remove_get0. eauto.
+      + inv CLOSED1. exploit CLOSED; eauto. i. des. splits; auto.
+        eapply future_closed_capability; eauto.
   Qed.
 
   Lemma promise_disjoint
         promises1 mem1 loc from to val released promises2 mem2 ctx kind
         (LE_PROMISES1: le promises1 mem1)
         (CLOSED1: closed mem1)
+        (CLOSED2: closed_capability released mem2)
         (PROMISE: promise promises1 mem1 loc from to val released promises2 mem2 kind)
         (LE_PROMISES: le ctx mem1)
         (DISJOINT: Memory.disjoint promises1 ctx):
@@ -1825,7 +958,6 @@ Module Memory.
   Lemma remove_future
         promises1 mem1 loc from to val released promises2
         (LE_PROMISES1: le promises1 mem1)
-        (CLOSED1: closed mem1)
         (REMOVE: remove promises1 loc from to val released promises2):
     <<LE_PROMISES2: le promises2 mem1>>.
   Proof.
@@ -1835,7 +967,6 @@ Module Memory.
   Lemma remove_disjoint
         promises1 mem1 loc from to val released promises2 ctx
         (LE_PROMISES1: le promises1 mem1)
-        (CLOSED1: closed mem1)
         (REMOVE: remove promises1 loc from to val released promises2)
         (LE_PROMISES: le ctx mem1)
         (DISJOINT: disjoint promises1 ctx):
@@ -1851,19 +982,34 @@ Module Memory.
   Lemma write_get2
         promises1 mem1 loc from to val released promises2 mem2 kind
         (PROMISES: le promises1 mem1)
-        (MEM: closed mem1)
+        (MEM: inhabited mem1)
         (WRITE: write promises1 mem1 loc from to val released promises2 mem2 kind):
     get loc to mem2 = Some (from, Message.mk val released).
   Proof.
     inv WRITE.
-    exploit promise_future; try apply PROMISE; eauto. i. des.
+    exploit promise_future0; try apply PROMISE; eauto. i. des.
     apply LE_PROMISES2. eapply promise_get2. eauto.
+  Qed.
+
+  Lemma write_future0
+        promises1 mem1 loc from to val released promises2 mem2 kind
+        (LE_PROMISES1: le promises1 mem1)
+        (INHABITED1: inhabited mem1)
+        (PROMISE: write promises1 mem1 loc from to val released promises2 mem2 kind):
+    <<LE_PROMISES2: le promises2 mem2>> /\
+    <<INHABITED2: inhabited mem2>> /\
+    <<FUTURE: future mem1 mem2>>.
+  Proof.
+    inv PROMISE.
+    hexploit promise_future0; eauto. i. des.
+    hexploit remove_future; eauto.
   Qed.
 
   Lemma write_future
         promises1 mem1 loc from to val released promises2 mem2 kind
         (LE_PROMISES1: le promises1 mem1)
         (CLOSED1: closed mem1)
+        (CLOSED2: closed_capability released mem2)
         (PROMISE: write promises1 mem1 loc from to val released promises2 mem2 kind):
     <<LE_PROMISES2: le promises2 mem2>> /\
     <<CLOSED2: closed mem2>> /\
@@ -1878,6 +1024,7 @@ Module Memory.
         promises1 mem1 loc from to val released promises2 mem2 ctx kind
         (LE_PROMISES1: le promises1 mem1)
         (CLOSED1: closed mem1)
+        (CLOSED2: closed_capability released mem2)
         (PROMISE: write promises1 mem1 loc from to val released promises2 mem2 kind)
         (LE_PROMISES: le ctx mem1)
         (DISJOINT: Memory.disjoint promises1 ctx):
@@ -2118,6 +1265,73 @@ Module Memory.
     { ii. eapply LE. eauto. }
     i. des.
     eexists. econs; eauto.
+  Qed.
+
+  Lemma get_lower
+        mem loc from to val released
+        (GET: get loc to mem = Some (from, Message.mk val released)):
+    lower mem loc from to val released released mem.
+  Proof.
+  Admitted.
+
+  Lemma add_lower_add
+        mem1 loc from to val released released' mem2
+        (ADD: add mem1 loc from to val released mem2)
+        (REL_LE: Capability.le released' released)
+        (REL_WF: Capability.wf released'):
+    exists mem2', add mem1 loc from to val released' mem2'.
+  Proof.
+    apply add_exists; auto.
+    - inv ADD. inv ADD0. eauto.
+    - inv ADD. inv ADD0. auto.
+  Qed.
+
+  Lemma split_lower_split
+        mem1 loc from to1 to2 val released released' mem2
+        (SPLIT: split mem1 loc from to1 to2 val released mem2)
+        (REL_LE: Capability.le released' released)
+        (REL_WF: Capability.wf released'):
+    exists mem2', split mem1 loc from to1 to2 val released' mem2'.
+  Proof.
+    exploit split_get0; eauto. i. des.
+    eapply split_exists; eauto.
+    - inv SPLIT. inv SPLIT0. auto.
+    - inv SPLIT. inv SPLIT0. auto.
+  Qed.
+
+  Lemma lower_lower_lower
+        mem1 loc from to val released0 released released' mem2
+        (LOWER: lower mem1 loc from to val released0 released mem2)
+        (REL_LE: Capability.le released' released)
+        (REL_WF: Capability.wf released'):
+    exists mem2', lower mem1 loc from to val released0 released' mem2'.
+  Proof.
+    inv LOWER.
+    exploit add_lower_add; eauto. i. des.
+    esplits. econs; eauto.
+    etrans; eauto.
+  Qed.
+
+  Lemma promise_lower_promise
+        promises1 mem1 loc from to val released released' promises2 mem2 kind
+        (PROMISE: promise promises1 mem1 loc from to val released promises2 mem2 kind)
+        (REL_LE: Capability.le released' released)
+        (REL_WF: Capability.wf released'):
+    exists promises2' mem2',
+      promise promises1 mem1 loc from to val released' promises2' mem2' kind.
+  Proof.
+    inv PROMISE.
+    - exploit add_lower_add; try apply PROMISES; eauto. i. des.
+      exploit add_lower_add; try apply MEM; eauto. i. des.
+      esplits. econs; eauto.
+      etrans; eauto. apply REL_LE.
+    - exploit split_lower_split; try apply PROMISES; eauto. i. des.
+      exploit split_lower_split; try apply MEM; eauto. i. des.
+      esplits. econs; eauto.
+      etrans; eauto. apply REL_LE.
+    - exploit lower_lower_lower; try apply PROMISES; eauto. i. des.
+      exploit lower_lower_lower; try apply MEM; eauto. i. des.
+      esplits. econs; eauto.
   Qed.
 
   Lemma promise_add_exists
