src/drf/PromiseIndep.v
@@ -9,6 +9,8 @@ Require Import DataStructure.
 Require Import Time.
 Require Import Event.
 Require Import Language.
+Require Import View.
+Require Import Cell.
 Require Import Memory.
 Require Import Commit.
 Require Import Thread.
