src/lang/Cell.v
@@ -1,0 +1,573 @@
+Require Import Omega.
+Require Import RelationClasses.
+
+Require Import sflib.
+Require Import paco.
+
+Require Import Axioms.
+Require Import Basic.
+Require Import DataStructure.
+Require Import DenseOrder.
+Require Import Event.
+Require Import Time.
+Require Import View.
+
+Set Implicit Arguments.
+
+
+Module Message.
+  Structure t := mk {
+    val: Const.t;
+    released: Capability.t;
+  }.
+  Definition elt: t := mk 0 Capability.bot.
+End Message.
+
+Module Cell.
+  Module Raw.
+    Definition t := DOMap.t (DenseOrder.t * Message.t).
+
+    Inductive wf (cell:t): Prop :=
+    | wf_intro
+        (VOLUME: forall from to msg
+                   (GET: DOMap.find to cell = Some (from, msg)),
+            (from, to) = (Time.bot, Time.bot) \/ Time.lt from to)
+        (DISJOINT: forall to1 to2 from1 from2 msg1 msg2
+                     (GET1: DOMap.find to1 cell = Some (from1, msg1))
+                     (GET2: DOMap.find to2 cell = Some (from2, msg2))
+                     (NEQ: to1 <> to2),
+            Interval.disjoint (from1, to1) (from2, to2))
+    .
+
+    Definition bot: t := DOMap.empty _.
+
+    Lemma bot_wf: wf bot.
+    Proof.
+      econs; i.
+      - rewrite DOMap.gempty in GET. inv GET.
+      - rewrite DOMap.gempty in GET1. inv GET1.
+    Qed.
+
+    Definition singleton (from to:Time.t) (val:Const.t) (released:Capability.t): t :=
+      DOMap.singleton to (from, Message.mk val released).
+
+    Lemma singleton_wf
+          from to val released
+          (LT: Time.lt from to):
+      wf (singleton from to val released).
+    Proof.
+      unfold singleton. econs; s; i.
+      - apply DOMap.singleton_find_inv in GET. des. inv GET0.
+        auto.
+      - apply DOMap.singleton_find_inv in GET1. des. inv GET0.
+        apply DOMap.singleton_find_inv in GET2. des. inv GET0.
+        congr.
+    Qed.
+
+    Definition init: t :=
+      DOMap.singleton Time.bot (Time.bot, Message.mk 0 Capability.bot).
+
+    Lemma init_wf: wf init.
+    Proof.
+      unfold init. econs; s; i.
+      - apply DOMap.singleton_find_inv in GET. des. inv GET0.
+        auto.
+      - apply DOMap.singleton_find_inv in GET1. des. inv GET0.
+        apply DOMap.singleton_find_inv in GET2. des. inv GET0.
+        congr.
+    Qed.
+
+    Lemma find_mem_ub
+          from to msg cell
+          (WF: wf cell)
+          (FIND: DOMap.find to cell = Some (from, msg)):
+      (from, to) = (Time.bot, Time.bot) \/
+      Interval.mem (from, to) to.
+    Proof.
+      inv WF. exploit VOLUME; eauto. i. des; auto.
+      right. econs; eauto. refl.
+    Qed.
+
+    Inductive add (cell1:t) (from to:Time.t) (val:Const.t) (released:Capability.t): forall (rhs:t), Prop :=
+    | add_intro
+        (DISJOINT: forall to2 from2 msg2
+                     (GET2: DOMap.find to2 cell1 = Some (from2, msg2)),
+            to <> from2 /\ Interval.disjoint (from, to) (from2, to2))
+        (TO1: Time.lt from to):
+        add cell1 from to val released (DOMap.add to (from, (Message.mk val released)) cell1)
+    .
+
+    Lemma add_wf
+          cell1 from to val released rhs
+          (ADD: add cell1 from to val released rhs)
+          (CELL1: wf cell1):
+      wf rhs.
+    Proof.
+      inv ADD. inv CELL1. econs; i.
+      - rewrite DOMap.Facts.add_o in *.
+        revert GET. condtac; i.
+        + inv GET. auto.
+        + eapply VOLUME. eauto.
+      - rewrite DOMap.Facts.add_o in *.
+        revert GET1 GET2. repeat condtac; i; repeat subst.
+        + congr.
+        + inv GET1. eapply DISJOINT; eauto.
+        + inv GET2. symmetry. eapply DISJOINT; eauto.
+        + eapply DISJOINT0; eauto.
+    Qed.
+
+    Inductive split (cell1:t) (from to1 to2:Time.t) (val1:Const.t) (released1:Capability.t): forall (rhs:t), Prop :=
+    | split_intro
+        msg2
+        (GET2: DOMap.find to2 cell1 = Some (from, msg2))
+        (TO1: Time.lt from to1)
+        (TO2: Time.lt to1 to2):
+        split cell1 from to1 to2 val1 released1
+              (DOMap.add to1 (from, Message.mk val1 released1) (DOMap.add to2 (to1, msg2) cell1))
+    .
+
+    Lemma split_wf
+          cell1 from1 to1 to2 val1 released1 cell2
+          (SPLIT: split cell1 from1 to1 to2 val1 released1 cell2)
+          (CELL1: wf cell1):
+      wf cell2.
+    Proof.
+      inv SPLIT. inv CELL1. econs; i.
+      - rewrite ? DOMap.Facts.add_o in *.
+        revert GET. repeat condtac; i; try by inv GET; auto.
+        eapply VOLUME. eauto.
+      - rewrite ? DOMap.Facts.add_o in *.
+        revert GET1 GET0. repeat condtac; i; repeat subst; try congr;
+          (repeat match goal with
+                 | [H: Some _ = Some _ |- _] => inv H
+                  end);
+          (try by eapply DISJOINT; eauto).
+        + apply Interval.disjoint_imm.
+        + ii. eapply (DISJOINT to3 to2); eauto.
+          eapply Interval.le_mem; try apply LHS.
+          econs; s. refl. apply Time.le_lteq. auto.
+        + symmetry. apply Interval.disjoint_imm.
+        + ii. eapply (DISJOINT to3 to0); eauto.
+          eapply Interval.le_mem; try apply LHS.
+          econs; s. apply Time.le_lteq. auto. refl.
+        + ii. eapply (DISJOINT to0 to2); eauto.
+          eapply Interval.le_mem; try apply RHS.
+          econs; s. refl. apply Time.le_lteq. auto.
+        + ii. eapply (DISJOINT to0 to3); eauto.
+          eapply Interval.le_mem; try apply RHS.
+          econs; s. apply Time.le_lteq. auto. refl.
+    Qed.
+
+    Inductive remove (cell1:t) (from to:Time.t) (val:Const.t) (released:Capability.t): forall (rhs:t), Prop :=
+    | remove_intro
+        (GET: DOMap.find to cell1 = Some (from, Message.mk val released)):
+        remove cell1 from to val released (DOMap.remove to cell1)
+    .
+
+    Lemma remove_wf
+          cell1 from to val released rhs
+          (REMOVE: remove cell1 from to val released rhs)
+          (CELL1: wf cell1):
+      wf rhs.
+    Proof.
+      inv REMOVE. inv CELL1. econs; i.
+      - revert GET0. rewrite DOMap.Facts.remove_o.
+        condtac; eauto. congr.
+      - revert GET1 GET2. rewrite ? DOMap.Facts.remove_o.
+        repeat condtac; i; try congr.
+        eapply DISJOINT; eauto.
+    Qed.
+  End Raw.
+
+  Structure t := mk {
+    raw :> Raw.t;
+    WF: Raw.wf raw;
+  }.
+
+  Definition get (ts:Time.t) (cell:t): option (Time.t * Message.t) := DOMap.find ts cell.(raw).
+
+  Lemma ext
+        (lhs rhs:t)
+        (EXT: forall ts, get ts lhs = get ts rhs):
+    lhs = rhs.
+  Proof.
+    destruct lhs, rhs.
+    assert (raw0 = raw1).
+    { apply DOMap.eq_leibniz. ii. apply EXT. }
+    subst raw1. f_equal. apply proof_irrelevance.
+  Qed.
+
+  Definition le (lhs rhs:t): Prop :=
+    forall to from msg
+      (LHS: get to lhs = Some (from, msg)),
+      get to rhs = Some (from, msg).
+
+  Global Program Instance le_PreOrder: PreOrder le.
+  Next Obligation. ii. auto. Qed.
+  Next Obligation. ii. eapply H0; eauto. Qed.
+
+  Inductive disjoint (lhs rhs:t): Prop :=
+  | disjoint_intro
+      (DISJOINT0: forall from1 from2 msg1 msg2
+                    (GET1: get Time.bot lhs = Some (from1, msg1))
+                    (GET2: get Time.bot rhs = Some (from2, msg2)),
+          False)
+      (DISJOINT1: forall to1 to2 from1 from2 msg1 msg2
+                    (GET1: get to1 lhs = Some (from1, msg1))
+                    (GET2: get to2 rhs = Some (from2, msg2)),
+          Interval.disjoint (from1, to1) (from2, to2))
+  .
+
+  Global Program Instance disjoint_Symmetric: Symmetric disjoint.
+  Next Obligation.
+    inv H. econs.
+    - i. eapply DISJOINT0; eauto.
+    - i. symmetry. eapply DISJOINT1; eauto.
+  Qed.
+
+  Lemma disjoint_get
+        lhs rhs
+        ts lmsg rmsg
+        (DISJOINT: disjoint lhs rhs)
+        (LMSG: get ts lhs = Some lmsg)
+        (RMSG: get ts rhs = Some rmsg):
+    False.
+  Proof.
+    destruct lmsg, rmsg. unfold get in *.
+    destruct (DOMap.find ts lhs.(raw)) as [[]|] eqn:LHS; inv LMSG.
+    destruct (DOMap.find ts rhs.(raw)) as [[]|] eqn:RHS; inv RMSG.
+    exploit Raw.find_mem_ub; try apply lhs; eauto. i.
+    exploit Raw.find_mem_ub; try apply rhs; eauto. i.
+    inv DISJOINT. des; inversion x0; inversion x1; subst; try by inv FROM.
+    - eapply DISJOINT0; eauto.
+    - eapply DISJOINT1; eauto.
+  Qed.
+
+  Definition bot: t := mk Raw.bot_wf.
+
+  Lemma bot_get ts: get ts bot = None.
+  Proof. unfold get, bot, Raw.bot. s. apply DOMap.gempty. Qed.
+
+  Lemma bot_le cell: le bot cell.
+  Proof. ii. rewrite bot_get in LHS. congr. Qed.
+
+  Lemma bot_disjoint cell: disjoint bot cell.
+  Proof.
+    econs.
+    - ii. rewrite bot_get in GET1. congr.
+    - i. rewrite bot_get in GET1. congr.
+  Qed.
+
+  Definition singleton
+             (from to:Time.t) (val:Const.t) (released:Capability.t)
+             (LT: Time.lt from to): t :=
+    mk (Raw.singleton_wf val released LT).
+
+  Lemma singleton_get
+        from to val released (LT:Time.lt from to)
+        t:
+    get t (singleton val released LT) =
+    if Loc.eq_dec t to
+    then Some (from, Message.mk val released)
+    else None.
+  Proof.
+    unfold get, singleton, Raw.singleton. ss. condtac.
+    - subst. rewrite DOMap.singleton_eq. auto.
+    - rewrite DOMap.singleton_neq; auto.
+  Qed.
+
+  Definition init: t := mk Raw.init_wf.
+
+  Definition add (cell1:t) (from1 to1:Time.t) (val1:Const.t) (released1:Capability.t) (cell2:t): Prop :=
+    Raw.add cell1 from1 to1 val1 released1 cell2.
+
+  Definition split (cell1:t) (from1 to1 to2:Time.t) (val1:Const.t) (released1:Capability.t) (cell2:t): Prop :=
+    Raw.split cell1 from1 to1 to2 val1 released1 cell2.
+
+  Definition remove (cell1:t) (from1 to1:Time.t) (val1:Const.t) (released1:Capability.t) (cell2:t): Prop :=
+    Raw.remove cell1 from1 to1 val1 released1 cell2.
+
+  Definition max_ts (cell:t): Time.t :=
+    DOMap.max_key _ cell.(raw).
+
+  Lemma max_ts_spec
+        ts from msg cell
+        (GET: get ts cell = Some (from, msg)):
+    <<GET: exists from val released, get (max_ts cell) cell = Some (from, Message.mk val released)>> /\
+    <<MAX: Time.le ts (max_ts cell)>>.
+  Proof.
+    unfold get in GET.
+    generalize (DOMap.max_key_spec _ cell.(Cell.raw)). i. des. splits; eauto.
+    - destruct (DOMap.find
+                  (DOMap.max_key (DenseOrder.t * Message.t) (Cell.raw cell))
+                  (Cell.raw cell)) as [[? []]|] eqn:X.
+      + esplits. eauto.
+      + exfalso. eapply FIND; eauto. rewrite GET. congr.
+    - apply MAX. rewrite GET. auto. congr.
+  Qed.
+
+  Lemma add_exists
+        cell1 from to val released
+        (DISJOINT: forall to2 from2 msg2
+                     (GET2: get to2 cell1 = Some (from2, msg2)),
+            to <> from2 /\ Interval.disjoint (from, to) (from2, to2))
+        (TO1: Time.lt from to):
+    exists cell2, add cell1 from to val released cell2.
+  Proof.
+    destruct cell1. eexists (mk _). unfold add. econs; eauto.
+  Grab Existential Variables.
+    eapply Raw.add_wf; eauto. econs; eauto.
+  Qed.
+
+  Lemma add_exists_max_ts
+        cell1 to val released
+        (TO: Time.lt (max_ts cell1) to)
+        (WF: Capability.wf released):
+    exists cell2, add cell1 (max_ts cell1) to val released cell2.
+  Proof.
+    apply add_exists; auto. i.
+    exploit max_ts_spec; eauto. i. des. splits.
+    - ii. subst. destruct cell1.(Cell.WF). exploit VOLUME; try apply GET2; eauto. i. des.
+      + inv x. inv TO.
+      + rewrite x in TO. eapply Time.lt_strorder. eapply TimeFacts.le_lt_lt; eauto.
+    - ii. inv LHS. inv RHS. ss.
+      rewrite MAX in TO1. eapply Time.lt_strorder. eapply TimeFacts.le_lt_lt; eauto.
+  Qed.
+
+  Lemma add_exists_le
+        promises1 cell1 from to val released cell2
+        (LE: le promises1 cell1)
+        (ADD: add cell1 from to val released cell2):
+    exists promises2, add promises1 from to val released promises2.
+  Proof.
+    inv ADD. apply add_exists; auto. i.
+    eapply DISJOINT. eauto.
+  Qed.
+
+  Lemma split_exists
+        cell1 from to1 to2 val released msg2
+        (GET2: get to2 cell1 = Some (from, msg2))
+        (TO1: Time.lt from to1)
+        (TO2: Time.lt to1 to2):
+    exists cell2, split cell1 from to1 to2 val released cell2.
+  Proof.
+    destruct cell1. eexists (mk _). unfold split. econs; eauto.
+  Grab Existential Variables.
+    eapply Raw.split_wf; eauto. econs; eauto.
+  Qed.
+
+  Lemma split_exists_le
+        promises1 cell1 from to1 to2 val released promises2
+        (LE: le promises1 cell1)
+        (SPLIT: split promises1 from to1 to2 val released promises2):
+    exists cell2, split cell1 from to1 to2 val released cell2.
+  Proof.
+    inv SPLIT. eapply split_exists; eauto.
+  Qed.
+
+  (* Lemmas on add, split & remove *)
+
+  Lemma add_disjoint
+        cell1 from1 to1 val1 released1 cell2
+        (ADD: add cell1 from1 to1 val1 released1 cell2):
+    get to1 cell1 = None.
+  Proof.
+    inv ADD. unfold get.
+    destruct (DOMap.find to1 (raw cell1)) as [[]|] eqn:X; auto.
+    exfalso. exploit DISJOINT; eauto. i. des.
+    eapply x0.
+    - apply Interval.mem_ub. auto.
+    - apply Interval.mem_ub.
+      destruct cell1.(Cell.WF). exploit VOLUME; eauto. i. des; ss.
+      inv x1. congr.
+  Qed.
+
+  Lemma add_get1
+        cell1 from1 to1 val1 released1 cell2
+        t f m
+        (ADD: add cell1 from1 to1 val1 released1 cell2)
+        (GET: get t cell1 = Some (f, m)):
+    get t cell2 = Some (f, m).
+  Proof.
+    exploit add_disjoint; eauto. i.
+    unfold get in *. inv ADD.
+    rewrite DOMap.gsspec. condtac; auto. subst.
+    congr.
+  Qed.
+
+  Lemma add_get2
+        cell1 from1 to1 val1 released1 cell2
+        (ADD: add cell1 from1 to1 val1 released1 cell2):
+    get to1 cell2 = Some (from1, Message.mk val1 released1).
+  Proof.
+    unfold get in *. inv ADD.
+    rewrite DOMap.gss. auto.
+  Qed.
+
+  Lemma add_get_inv
+        cell1 from1 to1 val1 released1 cell2
+        t f m
+        (ADD: add cell1 from1 to1 val1 released1 cell2)
+        (GET: get t cell2 = Some (f, m)):
+    (t = to1 /\ f = from1 /\ m = Message.mk val1 released1) \/
+    (~ t = to1 /\
+     get t cell1 = Some (f, m)).
+  Proof.
+    unfold get in *. inv ADD.
+    revert GET. rewrite <- H0. rewrite DOMap.gsspec. condtac; auto.
+    i. inv GET. auto.
+  Qed.
+
+  Lemma add_inhabited
+        cell1 cell2 from to val released
+        (ADD: add cell1 from to val released cell2)
+        (INHABITED: get Time.bot cell1 = Some (Time.bot, Message.elt)):
+    <<INHABITED: get Time.bot cell2 = Some (Time.bot, Message.elt)>>.
+  Proof.
+    des. exploit add_get1; eauto.
+  Qed.
+
+  Lemma add_max_ts
+        cell1 to val released cell2
+        (INHABITED: get Time.bot cell1 = Some (Time.bot, Message.elt))
+        (ADD: add cell1 (max_ts cell1) to val released cell2):
+    max_ts cell2 = to.
+  Proof.
+    hexploit add_inhabited; eauto. i. des.
+    exploit max_ts_spec; eauto. i. des.
+    apply TimeFacts.antisym.
+    - exploit add_get_inv; eauto. i. des.
+      + subst. refl.
+      + left. eapply TimeFacts.le_lt_lt.
+        * eapply max_ts_spec. rewrite x1. eauto.
+        * inv ADD. eauto.
+    - eapply max_ts_spec. erewrite add_get2; eauto.
+  Qed.
+
+  Lemma split_disjoint
+        cell1 from1 to1 to2 val1 released1 cell2
+        (SPLIT: split cell1 from1 to1 to2 val1 released1 cell2):
+    get to1 cell1 = None.
+  Proof.
+    unfold get in *. destruct cell1, cell2. inv SPLIT. ss. subst.
+    destruct (DOMap.find to1 raw0) as [[]|] eqn:X; [|done].
+    exfalso. inv WF0. eapply DISJOINT; [apply GET2|apply X| | |].
+    - ii. subst. eapply Time.lt_strorder. eauto.
+    - econs; eauto. apply Time.le_lteq. auto.
+    - apply Interval.mem_ub.
+      exploit VOLUME; eauto. i. des; ss.
+      inv x. inv TO1.
+  Qed.
+
+  Lemma split_get0
+        cell1 from1 to1 to2 val1 released1 cell2
+        (SPLIT: split cell1 from1 to1 to2 val1 released1 cell2):
+    exists msg2, get to2 cell1 = Some (from1, msg2).
+  Proof.
+    inv SPLIT. eauto.
+  Qed.
+
+  Lemma split_get1
+        cell1 from1 to1 to2 val1 released1 cell2
+        t f m
+        (SPLIT: split cell1 from1 to1 to2 val1 released1 cell2)
+        (GET: get t cell1 = Some (f, m)):
+    (f = from1 /\ t = to2 /\ get t cell2 = Some (to1, m)) \/
+    (~ (t = to2) /\
+     get t cell2 = Some (f, m)).
+  Proof.
+    unfold get in *. destruct cell1, cell2. inv SPLIT. ss. subst.
+    rewrite ? DOMap.gsspec. repeat condtac; subst; ss.
+    - destruct WF0.
+      exfalso. eapply DISJOINT; [apply GET2|apply GET| | |].
+      + ii. subst. eapply Time.lt_strorder. eauto.
+      + econs; eauto. apply Time.le_lteq. auto.
+      + apply Interval.mem_ub.
+        exploit VOLUME; eauto. i. des; ss.
+        inv x. inv TO1.
+    - rewrite GET2 in *. inv GET. eauto.
+    - rewrite GET. right. splits; eauto.
+  Qed.
+
+  Lemma split_get1'
+        cell1 from1 to1 to2 val1 released1 cell2
+        t f m
+        (SPLIT: split cell1 from1 to1 to2 val1 released1 cell2)
+        (GET: get t cell1 = Some (f, m)):
+    exists f', get t cell2 = Some (f', m).
+  Proof.
+    exploit split_get1; eauto. i. des; eauto.
+  Qed.
+
+  Lemma split_get2
+        cell1 from1 to1 to2 val1 released1 cell2
+        (SPLIT: split cell1 from1 to1 to2 val1 released1 cell2):
+    get to1 cell2 = Some (from1, Message.mk val1 released1).
+  Proof.
+    unfold get in *. destruct cell1, cell2. inv SPLIT. ss. subst.
+    apply DOMap.gss.
+  Qed.
+
+  Lemma split_get_inv
+        cell1 from1 to1 to2 val1 released1 cell2
+        t f m
+        (SPLIT: split cell1 from1 to1 to2 val1 released1 cell2)
+        (GET: get t cell2 = Some (f, m)):
+    (t = to1 /\ f = from1 /\ m = Message.mk val1 released1) \/
+    (t = to2 /\ f = to1 /\ get t cell1 = Some (from1, m)) \/
+    (~ (t = to1) /\
+     ~ (t = to2) /\
+     get t cell1 = Some (f, m)).
+  Proof.
+    unfold get in *. destruct cell1, cell2. inv SPLIT. ss. subst.
+    revert GET. rewrite ? DOMap.gsspec. repeat condtac; subst; i; inv GET; auto.
+  Qed.
+
+  Lemma split_get_inv'
+        cell1 from1 to1 to2 val1 released1 cell2
+        t f m
+        (SPLIT: split cell1 from1 to1 to2 val1 released1 cell2)
+        (GET: get t cell2 = Some (f, m)):
+    (t = to1 /\ f = from1 /\ m = Message.mk val1 released1) \/ exists f', get t cell1 = Some (f', m).
+  Proof.
+    exploit split_get_inv; eauto. i. des; eauto.
+  Qed.
+
+  Lemma split_inhabited
+        cell1 cell2 from to1 to2 val released
+        (SPLIT: split cell1 from to1 to2 val released cell2)
+        (INHABITED: get Time.bot cell1 = Some (Time.bot, Message.elt)):
+    <<INHABITED: get Time.bot cell2 = Some (Time.bot, Message.elt)>>.
+  Proof.
+    des. exploit split_get1; eauto. i. des; auto.
+    subst. inv SPLIT. inv TO2.
+  Qed.
+
+  Lemma remove_singleton
+        from to val released (LT:Time.lt from to):
+    remove (singleton val released LT) from to val released bot.
+  Proof.
+    assert (Raw.bot = DOMap.remove to ((singleton val released LT).(raw))).
+    { apply DOMap.eq_leibniz. ii.
+      unfold Raw.bot. rewrite DOMap.gempty.
+      rewrite DOMap.grspec. condtac; auto.
+      unfold singleton, Raw.singleton, raw.
+      rewrite DOMap.singleton_neq; auto.
+    }
+    unfold remove. s. rewrite H. econs. s.
+    unfold Raw.singleton. rewrite DOMap.singleton_eq. auto.
+  Qed.
+
+  Lemma remove_exists
+        cell1 from to val released
+        (GET: get to cell1 = Some (from, Message.mk val released)):
+    exists cell2, remove cell1 from to val released cell2.
+  Proof.
+    eexists (mk _). destruct cell1. ss.
+    Grab Existential Variables.
+    { eapply Raw.remove_wf.
+      - econs. eauto.
+      - apply WF.
+    }
+  Qed.
+End Cell.
