src/lang/View.v
@@ -1,0 +1,332 @@
+Require Import Omega.
+Require Import RelationClasses.
+
+Require Import sflib.
+Require Import paco.
+
+Require Import Axioms.
+Require Import Basic.
+Require Import DataStructure.
+Require Import DenseOrder.
+Require Import Event.
+Require Import Time.
+
+Set Implicit Arguments.
+
+
+Module TimeMap <: JoinableType.
+  Definition t := Loc.t -> Time.t.
+
+  Definition eq := @eq t.
+
+  Definition le (lhs rhs:t): Prop :=
+    forall loc, Time.le (lhs loc) (rhs loc).
+
+  Global Program Instance le_PreOrder: PreOrder le.
+  Next Obligation. ii. refl. Qed.
+  Next Obligation. ii. etrans; eauto. Qed.
+
+  Definition bot: t := fun _ => Time.bot.
+
+  Lemma bot_spec (tm:t): le bot tm.
+  Proof. ii. apply Time.bot_spec. Qed.
+
+  Definition get (loc:Loc.t) (c:t) := c loc.
+
+  Definition join (lhs rhs:t): t :=
+    fun loc => Time.join (lhs loc) (rhs loc).
+
+  Lemma join_comm lhs rhs: join lhs rhs = join rhs lhs.
+  Proof. apply LocFun.ext. i. apply Time.join_comm. Qed.
+
+  Lemma join_assoc a b c: join (join a b) c = join a (join b c).
+  Proof.
+    apply LocFun.ext. i. apply Time.join_assoc.
+  Qed.
+
+  Lemma join_l lhs rhs: le lhs (join lhs rhs).
+  Proof. ii. apply Time.join_l. Qed.
+
+  Lemma join_r lhs rhs: le rhs (join lhs rhs).
+  Proof. ii. apply Time.join_r. Qed.
+
+  Lemma join_spec lhs rhs o
+        (LHS: le lhs o)
+        (RHS: le rhs o):
+    le (join lhs rhs) o.
+  Proof. unfold join. ii. apply Time.join_spec; auto. Qed.
+
+  Definition singleton loc ts :=
+    LocFun.add loc ts (LocFun.init Time.bot).
+
+  Lemma singleton_spec loc ts c
+        (LOC: Time.le ts (c loc)):
+    le (singleton loc ts) c.
+  Proof.
+    ii. unfold singleton, LocFun.add, LocFun.find.
+    condtac; subst; ss. apply Time.bot_spec.
+  Qed.
+
+  Lemma singleton_inv loc ts c
+        (LE: le (singleton loc ts) c):
+    Time.le ts (c loc).
+  Proof.
+    generalize (LE loc). unfold singleton, LocFun.add, LocFun.find.
+    condtac; [|congr]. auto.
+  Qed.
+
+  Lemma le_join_l l r
+        (LE: le r l):
+    join l r = l.
+  Proof.
+    apply LocFun.ext. i.
+    unfold join, Time.join, LocFun.find. condtac; auto.
+    apply TimeFacts.antisym; auto.
+  Qed.
+
+  Lemma le_join_r l r
+        (LE: le l r):
+    join l r = r.
+  Proof.
+    apply LocFun.ext. i.
+    unfold join, Time.join, LocFun.find. condtac; auto.
+    exfalso. eapply Time.lt_strorder. eapply TimeFacts.lt_le_lt; eauto.
+  Qed.
+
+  Lemma antisym l r
+        (LR: le l r)
+        (RL: le r l):
+    l = r.
+  Proof.
+    extensionality loc. apply TimeFacts.antisym; auto.
+  Qed.
+End TimeMap.
+
+Module Capability <: JoinableType.
+  Structure t_ := mk {
+    ur: TimeMap.t;
+    rw: TimeMap.t;
+    sc: TimeMap.t;
+  }.
+  Definition t := t_.
+
+  Inductive wf (capability:t): Prop :=
+  | wf_intro
+      (UR_RW: TimeMap.le capability.(ur) capability.(rw))
+      (RW_SC: TimeMap.le capability.(rw) capability.(sc))
+  .
+
+  Definition eq := @eq t.
+
+  Inductive le_ (lhs rhs:t): Prop :=
+  | le_intro
+      (UR: TimeMap.le lhs.(ur) rhs.(ur))
+      (RW: TimeMap.le lhs.(rw) rhs.(rw))
+      (SC: TimeMap.le lhs.(sc) rhs.(sc))
+  .
+  Definition le := le_.
+
+  Global Program Instance le_PreOrder: PreOrder le.
+  Next Obligation.
+    ii. econs; refl.
+  Qed.
+  Next Obligation.
+    ii. inv H. inv H0. econs; etrans; eauto.
+  Qed.
+
+  Lemma ext l r
+        (UR: l.(ur) = r.(ur))
+        (RW: l.(rw) = r.(rw))
+        (SC: l.(sc) = r.(sc)):
+    l = r.
+  Proof.
+    destruct l, r. f_equal; auto.
+  Qed.
+
+  Definition bot: t := mk TimeMap.bot TimeMap.bot TimeMap.bot.
+
+  Lemma bot_wf: wf bot.
+  Proof. econs; refl. Qed.
+
+  Lemma bot_spec (c:t): le bot c.
+  Proof. econs; apply TimeMap.bot_spec. Qed.
+
+  Definition join (lhs rhs:t): t :=
+    mk (TimeMap.join lhs.(ur) rhs.(ur))
+       (TimeMap.join lhs.(rw) rhs.(rw))
+       (TimeMap.join lhs.(sc) rhs.(sc)).
+
+  Lemma join_comm lhs rhs: join lhs rhs = join rhs lhs.
+  Proof. unfold join. f_equal; apply TimeMap.join_comm. Qed.
+
+  Lemma join_assoc a b c: join (join a b) c = join a (join b c).
+  Proof.
+    unfold join. ss. f_equal.
+    - apply TimeMap.join_assoc.
+    - apply TimeMap.join_assoc.
+    - apply TimeMap.join_assoc.
+  Qed.
+
+  Lemma join_l lhs rhs: le lhs (join lhs rhs).
+  Proof. econs; apply TimeMap.join_l. Qed.
+
+  Lemma join_r lhs rhs: le rhs (join lhs rhs).
+  Proof. econs; apply TimeMap.join_r. Qed.
+
+  Lemma join_spec lhs rhs o
+        (LHS: le lhs o)
+        (RHS: le rhs o):
+    le (join lhs rhs) o.
+  Proof.
+    inv LHS. inv RHS.
+    econs; apply TimeMap.join_spec; eauto.
+  Qed.
+
+  Lemma join_wf
+        lhs rhs
+        (LHS: wf lhs)
+        (RHS: wf rhs):
+    wf (join lhs rhs).
+  Proof.
+    econs.
+    - apply TimeMap.join_spec.
+      + etrans; [apply LHS|]. apply TimeMap.join_l.
+      + etrans; [apply RHS|]. apply TimeMap.join_r.
+    - apply TimeMap.join_spec.
+      + etrans; [apply LHS|]. apply TimeMap.join_l.
+      + etrans; [apply RHS|]. apply TimeMap.join_r.
+  Qed.
+
+  Definition bot_unless (cond:bool) (c:t): t :=
+    if cond then c else bot.
+
+  Lemma bot_unless_wf
+        cond c
+        (WF: wf c):
+    wf (bot_unless cond c).
+  Proof.
+    destruct cond; ss. apply bot_wf.
+  Qed.
+
+  Definition singleton_ur loc ts :=
+    mk (TimeMap.singleton loc ts)
+       (TimeMap.singleton loc ts)
+       (TimeMap.singleton loc ts).
+
+  Lemma singleton_ur_wf
+        loc ts:
+    wf (singleton_ur loc ts).
+  Proof.
+    econs; ss; refl.
+  Qed.
+
+  Lemma singleton_ur_spec loc ts c
+        (WF: wf c)
+        (TS: Time.le ts (c.(ur) loc)):
+    le (singleton_ur loc ts) c.
+  Proof.
+    econs; s;
+      try apply TimeMap.bot_spec;
+      try apply TimeMap.singleton_spec; auto.
+    - etrans; eauto. apply WF.
+    - etrans; eauto. etrans; apply WF.
+  Qed.
+
+  Lemma singleton_ur_inv loc ts c
+        (LE: le (singleton_ur loc ts) c):
+    Time.le ts (c.(ur) loc).
+  Proof.
+    apply TimeMap.singleton_inv. apply LE.
+  Qed.
+
+  Definition singleton_rw loc ts :=
+    mk TimeMap.bot
+       (TimeMap.singleton loc ts)
+       (TimeMap.singleton loc ts).
+
+  Lemma singleton_rw_wf
+        loc ts:
+    wf (singleton_rw loc ts).
+  Proof.
+    econs; ss; try refl. apply TimeMap.bot_spec.
+  Qed.
+
+  Lemma singleton_rw_spec loc ts c
+        (WF: wf c)
+        (TS: Time.le ts (c.(rw) loc)):
+    le (singleton_rw loc ts) c.
+  Proof.
+    econs; s;
+      try apply TimeMap.bot_spec;
+      try apply TimeMap.singleton_spec; auto.
+    etrans; eauto. apply WF.
+  Qed.
+
+  Lemma singleton_rw_inv loc ts c
+        (LE: le (singleton_rw loc ts) c):
+    Time.le ts (c.(rw) loc).
+  Proof.
+    apply TimeMap.singleton_inv. apply LE.
+  Qed.
+
+  Definition singleton_sc loc ts :=
+    mk TimeMap.bot
+       TimeMap.bot
+       (TimeMap.singleton loc ts).
+
+  Lemma singleton_sc_wf
+        loc ts:
+    wf (singleton_sc loc ts).
+  Proof.
+    econs; ss; try refl. apply TimeMap.bot_spec.
+  Qed.
+
+  Lemma singleton_sc_spec loc ts c
+        (WF: wf c)
+        (TS: Time.le ts (c.(sc) loc)):
+    le (singleton_sc loc ts) c.
+  Proof.
+    econs; s;
+      try apply TimeMap.bot_spec;
+      try apply TimeMap.singleton_spec; auto.
+  Qed.
+
+  Lemma singleton_sc_inv loc ts c
+        (LE: le (singleton_sc loc ts) c):
+    Time.le ts (c.(sc) loc).
+  Proof.
+    apply TimeMap.singleton_inv. apply LE.
+  Qed.
+
+  Lemma le_join_l l r
+        (LE: le r l):
+    join l r = l.
+  Proof.
+    unfold join. destruct l. ss.
+    f_equal; apply TimeMap.le_join_l; apply LE.
+  Qed.
+
+  Lemma le_join_r l r
+        (LE: le l r):
+    join l r = r.
+  Proof.
+    unfold join. destruct r. ss.
+    f_equal; apply TimeMap.le_join_r; apply LE.
+  Qed.
+
+  Lemma antisym l r
+        (LR: le l r)
+        (RL: le r l):
+    l = r.
+  Proof.
+    destruct l, r. inv LR. inv RL. ss. f_equal.
+    - apply TimeMap.antisym; auto.
+    - apply TimeMap.antisym; auto.
+    - apply TimeMap.antisym; auto.
+  Qed.
+
+  Lemma timemap_le_le tm1 tm2
+        (LE: TimeMap.le tm1 tm2):
+    le (mk tm1 tm1 tm1) (mk tm2 tm2 tm2).
+  Proof. econs; eauto. Qed.
+End Capability.
